
\documentclass{article}
\usepackage{amsmath}
\usepackage{amssymb}
\usepackage{physics}

\begin{document}

\section*{Electrostatics Q1}

\subsection*{Part a}
Let $\vec{r} = z \hat{k}$ and $k = \frac{1}{4 \pi \epsilon_0}$.

\subsubsection*{Electric Field due to $q_1$}
\begin{align*}
\vec{E}_1 &= k \frac{q_1}{|\vec{r} - \vec{r}_1|^3} (\vec{r} - \vec{r}_1) \\
&= \frac{k q_1}{\left|z\hat{k} - (-\frac{d}{2})\hat{k}\right|^3} \left(z\hat{k} - (-\frac{d}{2})\hat{k}\right) \\
&= \frac{k q_1}{\left|z + \frac{d}{2}\right|^3} \left(z + \frac{d}{2}\right) \hat{k} \\
&= \frac{k q_1}{\left(z + \frac{d}{2}\right)^2} \frac{\left(z + \frac{d}{2}\right)}{\left|z + \frac{d}{2}\right|} \hat{k}
\end{align*}

\subsubsection*{Electric Field due to $q_2$}
\begin{align*}
\vec{E}_2 &= k \frac{q_2}{|\vec{r} - \vec{r}_2|^3} (\vec{r} - \vec{r}_2) \\
&= \frac{k q_2}{\left|z\hat{k} - (\frac{d}{2})\hat{k}\right|^3} \left(z\hat{k} - (\frac{d}{2})\hat{k}\right) \\
&= \frac{k q_2}{\left|z - \frac{d}{2}\right|^3} \left(z - \frac{d}{2}\right) \hat{k} \\
&= \frac{k q_2}{\left(z - \frac{d}{2}\right)^2} \frac{\left(z - \frac{d}{2}\right)}{\left|z - \frac{d}{2}\right|} \hat{k}
\end{align*}

\subsection*{By superposition principle: $\vec{E} = \vec{E}_1 + \vec{E}_2$}

\subsection*{Case 1: $z > \frac{d}{2}$}
\begin{align*}
\vec{E} &= \vec{E}_1 + \vec{E}_2 \\
&= \frac{k q_1}{\left(z + \frac{d}{2}\right)^2}  \hat{k} + \frac{k q_2}{\left(z - \frac{d}{2}\right)^2} \hat{k} \\
&= \left( \frac{k q_1}{\left(z + \frac{d}{2}\right)^2} + \frac{k q_2}{\left(z - \frac{d}{2}\right)^2} \right) \hat{k}
\end{align*}

Since $q_1 = q_2 = q$,
\begin{align*}
\vec{E} &= k q \left[ \frac{1}{\left(z + \frac{d}{2}\right)^2} + \frac{1}{\left(z - \frac{d}{2}\right)^2} \right] \hat{k}
\end{align*}

\subsection*{Case 2: $-\frac{d}{2} < z < \frac{d}{2}$}
\begin{align*}
\vec{E} &= \vec{E}_1 + \vec{E}_2 \\
&= \frac{k q_1}{\left(z + \frac{d}{2}\right)^2} \hat{k} + \frac{k q_2}{\left(z - \frac{d}{2}\right)^2} (-\hat{k}) \\
&= k q \left[ \frac{1}{\left(z + \frac{d}{2}\right)^2} - \frac{1}{\left(z - \frac{d}{2}\right)^2} \right] \hat{k}
\end{align*}

\subsection*{Case 3: $z < -\frac{d}{2}$}
\begin{align*}
\vec{E} &= \vec{E}_1 + \vec{E}_2 \\
&= \frac{k q_1}{\left(z + \frac{d}{2}\right)^2} (-\hat{k}) + \frac{k q_2}{\left(z - \frac{d}{2}\right)^2} (-\hat{k}) \\
&= -k q \left[ \frac{1}{\left(z + \frac{d}{2}\right)^2} + \frac{1}{\left(z - \frac{d}{2}\right)^2} \right] \hat{k}
\end{align*}

\end{document}

